deriving/test/Test.lean
@@ -1,0 +1,13 @@
+/-
+Copyright (c) 2026 Paul Butcher. All rights reserved.
+Released under Apache 2.0 license as described in the file LICENSE.
+-/
+import Test.Runner
+import Test.Codecs
+import Test.Syntax
+
+namespace Test
+
+def all : Array TestCase := Test.Codecs.all ++ Test.Syntax.all
+
+end Test
