deriving/test/lakefile.lean
@@ -1,0 +1,21 @@
+/-
+Copyright (c) 2026 Paul Butcher. All rights reserved.
+Released under Apache 2.0 license as described in the file LICENSE.
+-/
+import Lake
+open Lake DSL
+
+package test where
+  leanOptions := #[⟨`warningAsError, true⟩]
+
+require jsonDeriving from ".."
+
+require plausible from git
+  "https://github.com/leanprover-community/plausible" @ "v4.33.0"
+
+@[default_target]
+lean_lib Test
+
+@[test_driver]
+lean_exe runTests where
+  root := `Main
